theories/ml_lang/proofmode.v
@@ -23,7 +23,7 @@ Ltac solve_lookup_fixed := let rec go := match goal with
     (unify key needle; rewrite (@lookup_singleton _ _ _ _ _ _ _ _ _ _ _ _ key val)) ||
     (rewrite (@lookup_singleton_ne _ _ _ _ _ _ _ _ _ _ _ _ key needle val); congruence)
 | [ |- context[ @lookup _ _ (@gmap _ ?eqdec _ _) _ ?needle ∅]] => 
-    rewrite (@lookup_empty _ _  _ _ _ _ _ _ _ _ _ _ needle) end in repeat (progress (unfold subst; try go; simpl)).
+    rewrite (@lookup_empty _ _  _ _ _ _ _ _ _ _ _ _ needle) end in repeat (progress (unfold subst; try go; cbn)).
 
 Tactic Notation "wp_expr_eval" tactic3(t) :=
   iStartProof;
